SStructTT/Static/Step.lean
@@ -7,88 +7,88 @@ variable {Srt : Type}
 
 @[aesop safe [constructors]]
 inductive Step : Tm Srt -> Tm Srt -> Prop where
-  | piA {A A' B r s} :
+  | piA {A A'} B r s :
     Step A A' ->
     Step (.pi A B r s) (.pi A' B r s)
-  | piB {A B B' r s} :
+  | piB A {B B'} r s :
     Step B B' ->
     Step (.pi A B r s) (.pi A B' r s)
-  | lamA {A A' m r s} :
+  | lamA {A A'} m r s :
     Step A A' ->
     Step (.lam A m r s) (.lam A' m r s)
-  | lamM {A m m' r s} :
+  | lamM A {m m'} r s :
     Step m m' ->
     Step (.lam A m r s) (.lam A m' r s)
-  | appM {m m' n} :
+  | appM {m m'} n :
     Step m m' ->
     Step (.app m n) (.app m' n)
-  | appN {m n n'} :
+  | appN m {n n'} :
     Step n n' ->
     Step (.app m n) (.app m n')
-  | beta {A m n r s} :
+  | beta A m n r s :
     Step (.app (.lam A m r s) n) m.[n/]
-  | sigA {A A' B r s} :
+  | sigA {A A'} B r s :
     Step A A' ->
     Step (.sig A B r s) (.sig A' B r s)
-  | sigB {A B B' r s} :
+  | sigB A {B B'} r s :
     Step B B' ->
     Step (.sig A B r s) (.sig A B' r s)
-  | pairM {m m' n r s} :
+  | pairM {m m'} n r s :
     Step m m' ->
     Step (.pair m n r s) (.pair m' n r s)
-  | pairN {m n n' r s} :
+  | pairN m {n n'} r s :
     Step n n' ->
     Step (.pair m n r s) (.pair m n' r s)
-  | projA {A A' m n} :
+  | projA {A A'} m n :
     Step A A' ->
     Step (.proj A m n) (.proj A' m n)
-  | projM {A m m' n} :
+  | projM A {m m'} n :
     Step m m' ->
     Step (.proj A m n) (.proj A m' n)
-  | projN {A m n n'} :
+  | projN A m {n n'} :
     Step n n' ->
     Step (.proj A m n) (.proj A m n')
-  | projE {A m1 m2 n r s} :
+  | projE A m1 m2 n r s :
     Step (.proj A (.pair m1 m2 r s) n) n.[m2,m1/]
-  | iteA {A A' m n1 n2} :
+  | iteA {A A'} m n1 n2 :
     Step A A' ->
     Step (.ite A m n1 n2) (.ite A' m n1 n2)
-  | iteM {A m m' n1 n2} :
+  | iteM A {m m'} n1 n2 :
     Step m m' ->
     Step (.ite A m n1 n2) (.ite A m' n1 n2)
-  | iteN1 {A m n1 n1' n2} :
+  | iteN1 A m {n1 n1'} n2 :
     Step n1 n1' ->
     Step (.ite A m n1 n2) (.ite A m n1' n2)
-  | iteN2 {A m n1 n2 n2'} :
+  | iteN2 A m n1 {n2 n2'} :
     Step n2 n2' ->
     Step (.ite A m n1 n2) (.ite A m n1 n2')
-  | iteT {A n1 n2} :
+  | iteT A n1 n2 :
     Step (.ite A .tt n1 n2) n1
-  | iteF {A n1 n2} :
+  | iteF A n1 n2 :
     Step (.ite A .ff n1 n2) n2
-  | idA {A A' m n} :
+  | idA {A A'} m n :
     Step A A' ->
     Step (.id A m n) (.id A' m n)
-  | idM {A m m' n} :
+  | idM A {m m'} n :
     Step m m' ->
     Step (.id A m n) (.id A m' n)
-  | idN {A m n n'} :
+  | idN A m {n n'} :
     Step n n' ->
     Step (.id A m n) (.id A m n')
   | rflM {m m'} :
     Step m m' ->
     Step (.rfl m) (.rfl m')
-  | rwA {A A' m n} :
+  | rwA {A A'} m n :
     Step A A' ->
     Step (.rw A m n) (.rw A' m n)
-  | rwM {A m m' n} :
+  | rwM A {m m'} n :
     Step m m' ->
     Step (.rw A m n) (.rw A m' n)
-  | rwN {A m n n'} :
+  | rwN A m {n n'} :
     Step n n' ->
     Step (.rw A m n) (.rw A m n')
-  | rwE {A m n} :
-    Step (.rw A m (.rfl n)) n
+  | rwE A m n :
+    Step (.rw A m (.rfl n)) m
 
 @[reducible]def StarStep := Star (@Step Srt)
 @[reducible]def ConvStep := Conv (@Step Srt)
